merkle: move pure things to theory file

new/proof/github_com/sanjit_bhat/pav/merkle_proof/code.v
@@ -787,6 +787,34 @@ Proof.
   by simplify_eq/=.
 Qed.
 
+(* invariants on proofToTree tree that allow subsequent puts.
+some invs established with additional info in wish,
+which is why we make it the precond. *)
+Lemma proofToTree_post label proof_enc t :
+  wish_proofToTree label proof_enc t -∗
+  ("%Hlabel_None" ∷ ⌜is_entry t label None⌝ ∗
+  "%Hcutless" ∷ ⌜is_cutless_path t label⌝ ∗
+  "%Hlimit" ∷ ⌜is_limit t⌝ ∗
+  "%Hsorted" ∷ ⌜is_sorted t⌝ ∗
+  "%Hconst_label_len" ∷ ⌜is_const_label_len t⌝).
+Proof.
+  iIntros "@".
+  opose proof (newShell_None label sibs).
+  opose proof (cutless_on_newShell label sibs).
+  opose proof (limit_on_newShell label sibs _); [word|].
+  opose proof (sorted_on_newShell label sibs).
+  opose proof (const_label_on_newShell label sibs).
+  destruct oleaf as [[]|]; simplify_eq/=; [|done].
+  iNamed "Holeaf".
+
+  eapply old_entry_over_put in Hcode as ?; [|done..].
+  eapply cutless_path_over_put in Hcode as ?; [|done].
+  eapply is_limit_over_put in Hcode as ?; [|done].
+  eapply is_sorted_over_put in Hcode as ?; [|done].
+  eapply const_label_len_over_put in Hcode as ?; [|done|word].
+  by opose proof (put_impl_cutless_pre _ _ _ _).
+Qed.
+
 Tactic Notation "intro_wish" := iIntros "(%&%&@)".
 
 Lemma wp_proofToTree sl_label label sl_proof proof :
@@ -804,15 +832,7 @@ Lemma wp_proofToTree sl_label label sl_proof proof :
       | false =>
         ∃ t,
         "Hwish" ∷ wish_proofToTree label proof t ∗
-        "Hown_tree" ∷ own_tree tr t 1 ∗
-
-        (* TODO: rm after prove wish_toTree lemma. *)
-        (* necessary for subsequent put's. *)
-        "%Hlabel_None" ∷ ⌜is_entry t label None⌝ ∗
-        "%Hcutless" ∷ ⌜is_cutless_path t label⌝ ∗
-        "%Hlimit" ∷ ⌜is_limit t⌝ ∗
-        "%Hsorted" ∷ ⌜is_sorted t⌝ ∗
-        "%Hconst_label_len" ∷ ⌜is_const_label_len t⌝
+        "Hown_tree" ∷ own_tree tr t 1
       end
   }}}.
 Proof.
@@ -852,11 +872,6 @@ Proof.
   destruct obj. simplify_eq/=.
   rewrite join_length_reverse in Hlen_sl_sibs.
   apply join_same_len_length in Hlen_sibs as ?.
-  opose proof (newShell_None label sibs).
-  opose proof (cutless_on_newShell label sibs).
-  opose proof (limit_on_newShell label sibs _); [word|].
-  opose proof (sorted_on_newShell label sibs).
-  opose proof (const_label_on_newShell label sibs).
   replace (pure_newShell' _ _ _) with (pure_newShell label sibs) by done.
 
   destruct IsOtherLeaf; wp_auto.
@@ -902,17 +917,10 @@ Proof.
     { word. }
     apply (inj _) in Heq_s.
     simplify_eq/=. iApply "Hgenie". iPureIntro.
-    by eapply put_impl_cutless. }
+    by eapply put_impl_cutless_pre. }
 
   iApply "HΦ".
   iFrame "Hown_tree".
-  eapply old_entry_over_put in Hcode as ?; [|done..].
-  eapply cutless_over_put in Hcode as ?; [|done].
-  eapply is_limit_over_put in Hcode as ?; [|done].
-  eapply is_sorted_over_put in Hcode as ?; [|done].
-  eapply const_label_len_over_put in Hcode as ?; [|done|word].
-  opose proof (put_impl_cutless _ _ _ _); [done|].
-  repeat iSplit; [|done..].
   iExists _, (Some (_, _)).
   iFrame. iPureIntro. repeat split; try done; word.
 Qed.
@@ -920,38 +928,6 @@ Qed.
 (* make defn to prevent unfolding the nat. *)
 Definition w64_len := 8%nat.
 Hint Unfold w64_len : word.
-
-(* very similar to [to_map_Some]. *)
-Lemma is_sorted_find_pref t pref label fl fv :
-  find' t (length pref) label = Some (fl, fv) →
-  is_sorted' t pref →
-  prefix_total pref (bytes_to_bits fl).
-Proof.
-  revert pref.
-  induction t; simpl; intros; simplify_eq/=; try done.
-  intuition.
-  replace (S _) with (length (pref ++
-    [if get_bit label (length pref) then true else false])) in * by len.
-  case_match.
-  - eapply prefix_total_app_l.
-    by eapply IHt2.
-  - eapply prefix_total_app_l.
-    by eapply IHt1.
-Qed.
-
-Lemma find_to_bit_eq t0 t1 pref label fl fv :
-  find' (Inner t0 t1) (length pref) label = Some (fl, fv) →
-  is_sorted' t0 (pref ++ [false]) →
-  is_sorted' t1 (pref ++ [true]) →
-  get_bit label (length pref) = get_bit fl (length pref).
-Proof.
-  simpl. intros Hf **.
-  replace (S _) with (length (pref ++ [get_bit label (length pref)])) in Hf by len.
-  eapply is_sorted_find_pref in Hf.
-  2: { by case_match. }
-  eapply prefix_total_snoc_inv in Hf.
-  intuition.
-Qed.
 
 Lemma wp_node_find n t d0 sl_label d1 label (getProof : bool) :
   (* limit needed to prevent depth overflow. *)
@@ -1237,6 +1213,7 @@ Proof.
     iDestruct own_slice_nil as "$".
     intro_wish. iApply "Hgenie". iFrame. }
   iNamed "Hgenie".
+  iDestruct (proofToTree_post with "[$]") as "#@".
   iNamed "Hwish".
 
   wp_apply (wp_put with "[$tr $Hown_tree]") as "* @"; try done.
@@ -1316,6 +1293,7 @@ Proof.
     iDestruct own_slice_nil as "$".
     intro_wish. iApply "Hgenie". iFrame. }
   iNamed "Hgenie".
+  iDestruct (proofToTree_post with "[$]") as "#@".
   iNamed "Hwish".
 
   wp_apply (wp_node_getHash with "[$Hown_tree]") as "*".
@@ -1357,18 +1335,6 @@ Proof.
       by eapply old_entry_over_put.
   - rewrite -entry_eq_lookup.
     by iApply full_entry_txfer; [..|by iFrame "#"].
-Qed.
-
-Lemma find_on_const_label_len t label l v :
-  find t label = Some (l, v) →
-  is_const_label_len t →
-  Z.of_nat (length l) = cryptoffi.hash_len.
-Proof.
-  autounfold with merkle.
-  remember 0%nat as depth. clear Heqdepth.
-  revert t depth.
-  induction t; intros; simplify_eq/=; try done.
-  case_match; naive_solver.
 Qed.
 
 Lemma wp_node_prove n t d0 sl_label d1 label getProof :
@@ -1643,17 +1609,6 @@ Proof.
   iFrame "∗#%".
 Qed.
 
-Lemma is_cutless_to_path t label :
-  is_cutless t →
-  is_cutless_path t label.
-Proof.
-  autounfold with merkle.
-  remember 0%nat as depth. clear Heqdepth.
-  revert depth.
-  induction t; intros; simplify_eq/=; try done.
-  case_match; naive_solver.
-Qed.
-
 Lemma wp_Map_Prove ptr m hash d0 sl_label d1 label :
   {{{
     is_pkg_init merkle ∗
@@ -1696,226 +1651,6 @@ Proof.
   subst.
   iApply "HΦ".
   by iFrame "∗#%".
-Qed.
-
-Lemma put_impl_non_cut t depth label val limit :
-  is_Some (pure_put' t depth label val limit) →
-  ∀ h, t ≠ Cut h.
-Proof. rewrite pure_put_unfold. by destruct t. Qed.
-
-Definition cut_cut_reln t0 t1 h : iProp Σ :=
-  "#Ht0" ∷ is_cut_tree t0 h ∗
-  "#Ht1" ∷ is_cut_tree t1 h.
-
-Lemma cut_cut_reln_Empty t h :
-  cut_cut_reln Empty t h -∗
-  ⌜∀ h, t ≠ Cut h⌝ -∗
-  ⌜t = Empty⌝.
-Proof.
-  iIntros "@ %Hpath".
-  destruct t; simpl; try naive_solver;
-    iNamedSuffix "Ht0" "0";
-    iNamedSuffix "Ht1" "1";
-    by iDestruct (cryptoffi.is_hash_inj with "His_hash0 His_hash1") as %?.
-Qed.
-
-Lemma cut_cut_reln_Leaf l v t h :
-  cut_cut_reln (Leaf l v) t h -∗
-  ⌜∀ h, t ≠ Cut h⌝ -∗
-  ⌜t = Leaf l v⌝.
-Proof.
-  iIntros "@ %Hpath".
-  destruct t; simpl; try naive_solver;
-    iNamedSuffix "Ht0" "0";
-    iNamedSuffix "Ht1" "1";
-    iDestruct (cryptoffi.is_hash_inj with "His_hash0 His_hash1") as %Henc;
-    try done.
-  iPureIntro.
-  list_simplifier.
-  apply app_inj_1 in Henc as [Hlen_label Henc]; [|len].
-  apply (inj u64_le) in Hlen_label.
-  apply app_inj_1 in Henc as [<- Henc]; [|word].
-  by apply app_inj_1 in Henc as [_ <-]; [|len].
-Qed.
-
-Lemma cut_cut_reln_Inner c0 c1 t h :
-  cut_cut_reln (Inner c0 c1) t h -∗
-  ⌜∀ h, t ≠ Cut h⌝ -∗
-  ∃ c0' c1' h0 h1,
-  ⌜t = Inner c0' c1'⌝ ∗
-  cut_cut_reln c0 c0' h0 ∗
-  cut_cut_reln c1 c1' h1.
-Proof.
-  iIntros "@ %Hpath".
-  destruct t; simpl; try naive_solver;
-    iNamedSuffix "Ht0" "_l";
-    iNamedSuffix "Ht1" "_r";
-    iDestruct (cryptoffi.is_hash_inj with "His_hash_l His_hash_r") as %Henc;
-    try done.
-  list_simplifier.
-  iDestruct (is_cut_tree_len with "Hchild0_l") as %?.
-  iDestruct (is_cut_tree_len with "Hchild1_l") as %?.
-  iDestruct (is_cut_tree_len with "Hchild0_r") as %?.
-  iDestruct (is_cut_tree_len with "Hchild1_r") as %?.
-  apply app_inj_1 in Henc as [<- <-]; [|word].
-  repeat iExists _.
-  iSplit; [done|].
-  iFrame "#".
-Qed.
-
-Lemma cut_cut_hash_over_put t0 t1 h label val t0' t1' h' :
-  cut_cut_reln t0 t1 h -∗
-  ⌜pure_put t0 label val = Some t0'⌝ -∗
-  ⌜pure_put t1 label val = Some t1'⌝ -∗
-  is_cut_tree t0' h' -∗
-  is_cut_tree t1' h'.
-Proof.
-  autounfold with merkle.
-  remember max_depth as limit. clear Heqlimit.
-  remember 0%nat as depth. clear Heqdepth.
-  iInduction limit as [? IH] using lt_wf_ind forall (t0 t1 h t0' t1' h' depth).
-  iIntros "#Hreln %Hput0 %Hput1 #Hhash_t0'".
-  rewrite pure_put_unfold in Hput0.
-
-  destruct t0; try done.
-  - iDestruct (cut_cut_reln_Empty with "Hreln [%]") as %->.
-    { by eapply put_impl_non_cut. }
-    rewrite pure_put_unfold in Hput1.
-    simplify_eq/=.
-    iFrame "#".
-  - iDestruct (cut_cut_reln_Leaf with "Hreln [%]") as %->.
-    { by eapply put_impl_non_cut. }
-    rewrite pure_put_unfold in Hput1.
-    case_decide.
-    { simplify_eq/=. iFrame "#". }
-    case_match; try done.
-    simpl in *.
-    case_match; try done.
-    simplify_eq/=.
-    iFrame "#".
-  - iDestruct (cut_cut_reln_Inner with "Hreln [%]") as "(%&%&%&%&->&#Hreln0&#Hreln1)".
-    { by eapply put_impl_non_cut. }
-    rewrite pure_put_unfold in Hput1.
-    case_match; try done.
-    simpl in *.
-    destruct (pure_put' _ _ _ _ _) eqn:? in Hput0; try done.
-    destruct (pure_put' _ _ _ _ _) eqn:? in Hput1; try done.
-    simplify_eq/=.
-    iSpecialize ("IH" $! n with "[]"); [word|].
-    iNamed "Hhash_t0'".
-    case_match.
-    + iDestruct ("IH" with "Hreln1 [//][//][$]") as "$".
-      iNamed "Hreln0".
-      iDestruct (is_cut_tree_det with "Hchild0 Ht0") as %->.
-      iFrame "#".
-    + iDestruct ("IH" with "Hreln0 [//][//][$]") as "$".
-      iNamed "Hreln1".
-      iDestruct (is_cut_tree_det with "Hchild1 Ht0") as %->.
-      iFrame "#".
-Qed.
-
-Tactic Notation "rw_pure_put" := repeat
-  match goal with
-  | H : pure_put' _ _ _ _ _ = None |- _ => rewrite -{}H
-  end.
-
-Lemma put_Some t label val :
-  (* for max depth. *)
-  is_limit t →
-  Z.of_nat (length label) = cryptoffi.hash_len →
-  is_const_label_len t →
-  is_sorted t →
-  (* for no Cut. *)
-  is_cutless_path t label →
-  is_Some (pure_put t label val).
-Proof.
-  autounfold with merkle.
-  assert (∃ x, x = max_depth) as [limit Heq]; [by eexists|].
-  rewrite -[in is_limit' _ _]Heq.
-  rewrite -[in pure_put' _ _ _ _ _]Heq.
-  remember [] as pref.
-  assert (prefix_total pref (bytes_to_bits label)).
-  { subst. apply prefix_total_nil. }
-  replace 0%nat with (length pref); [|by subst].
-  assert (length pref + limit = max_depth)%nat.
-  { subst. simpl. lia. }
-  clear Heq Heqpref.
-  intros.
-  generalize dependent t.
-  generalize dependent pref.
-
-  induction limit as [? IH] using lt_wf_ind.
-  intros. rewrite pure_put_unfold.
-  destruct t; simpl in *; try done.
-
-  - case_decide; [done|].
-    destruct limit.
-    (* limit=0. show labels actually equal. *)
-    { opose proof (prefix_total_full _ (bytes_to_bits label) _ _);
-        [|done|]; [by len|].
-      opose proof (prefix_total_full _ (bytes_to_bits label0) _ _);
-        [|done|]; [by len|].
-      simplify_eq/=. }
-
-    ospecialize (IH limit _); [lia|].
-    destruct (pure_put' _ _ _ _ _) eqn:?; [done|]. rw_pure_put.
-    replace (S _) with (length $ pref_ext pref label) in * by len.
-    eapply IH; repeat case_match; try done; [|len|..];
-      by eapply prefix_total_snoc.
-  - destruct limit; [done|].
-    ospecialize (IH limit _); [lia|].
-    intuition.
-    destruct (pure_put' _ _ _ _ _) eqn:?; [done|]. rw_pure_put.
-    replace (S _) with (length $ pref_ext pref label) in * by len.
-    eapply IH; repeat case_match; try done; [..|len|len];
-      by eapply prefix_total_snoc.
-Qed.
-
-Lemma proofToTree_to_put_precond label proof_enc t :
-  wish_proofToTree label proof_enc t -∗
-  ("%Hlabel_None" ∷ ⌜is_entry t label None⌝ ∗
-  "%Hcutless" ∷ ⌜is_cutless_path t label⌝ ∗
-  "%Hlimit" ∷ ⌜is_limit t⌝ ∗
-  "%Hsorted" ∷ ⌜is_sorted t⌝ ∗
-  "%Hconst_label_len" ∷ ⌜is_const_label_len t⌝).
-Proof.
-  iIntros "@".
-  opose proof (newShell_None label sibs).
-  opose proof (cutless_on_newShell label sibs).
-  opose proof (limit_on_newShell label sibs _); [word|].
-  opose proof (sorted_on_newShell label sibs).
-  opose proof (const_label_on_newShell label sibs).
-  destruct oleaf as [[]|]; simplify_eq/=; [|done].
-  iNamed "Holeaf".
-
-  eapply old_entry_over_put in Hcode as ?; [|done..].
-  eapply cutless_over_put in Hcode as ?; [|done].
-  eapply is_limit_over_put in Hcode as ?; [|done].
-  eapply is_sorted_over_put in Hcode as ?; [|done].
-  eapply const_label_len_over_put in Hcode as ?; [|done|word].
-  by opose proof (put_impl_cutless _ _ _ _).
-Qed.
-
-(* TODO: name conflict. *)
-Lemma is_cutless_over_put t label val t' :
-  is_cutless t →
-  pure_put t label val = Some t' →
-  is_cutless t'.
-Proof.
-  autounfold with merkle.
-  remember max_depth as limit. clear Heqlimit.
-  remember 0%nat as depth. clear Heqdepth.
-  revert t t' depth.
-  induction limit as [? IH] using lt_wf_ind.
-  intros *. rewrite pure_put_unfold.
-  destruct t; simpl; intros;
-    try case_decide; try case_match; try case_match;
-    simplify_eq/=; try done.
-  - ospecialize (IH n _); [lia|].
-    repeat case_match; intuition;
-      (by eapply IH; [|done]).
-  - ospecialize (IH n _); [lia|].
-    repeat case_match; intuition; (by eapply IH; [|done]).
 Qed.
 
 Lemma wp_Map_Put ptr m hash sl_label label sl_val val :
@@ -1968,7 +1703,7 @@ Proof.
   iFrame. iSplit.
   - iFrame "#". iPureIntro. repeat split.
     + symmetry. by eapply to_map_over_put.
-    + by eapply is_cutless_over_put.
+    + by eapply cutless_over_put.
     + by eapply is_limit_over_put.
     + eapply const_label_len_over_put; try done. word.
     + by eapply is_sorted_over_put.
